Towards environment separation

theories/Environment.v
@@ -5,6 +5,7 @@ From MailboxTypes Require Import Util.
 
 Require Import Lists.List.
 Import ListNotations.
+Require Import Lia.
 
 Generalizable All Variables.
 
@@ -22,7 +23,7 @@ Context `{M : IMessage Message}.
     3 |-> None
 
    This represented is chosen to keep avoid shifting de Bruijn indices
-   when splitting an environment.
+when splitting an environment.
 *)
 Definition Env := list (option TUsage).
 
@@ -157,6 +158,13 @@ Fixpoint SingletonEnv (e : Env) : Prop :=
   | (Some _) :: e' => EmptyEnv e'
   end.
 
+(** Creates an empty environment based on the size of the provided environment *)
+Fixpoint create_EmptyEnv (e : Env) : Env :=
+  match e with
+  | nil => nil
+  | t :: e' => None :: create_EmptyEnv e'
+  end.
+
 End environment_def.
 
 (** Notation for environments *)
@@ -172,8 +180,519 @@ Notation "[ Env1 ]+ₑ ~= Env" := (EnvironmentDisjointCombinationN Env1 Env) (at
 Notation "⌊ Env ⌋ₑ" := (returnEnvironment Env) : environment_scope.
 Notation "⌈ Env ⌉ₑ" := (secondEnvironment Env) : environment_scope.
 
+Section environment_test.
+
+Context `{M : IMessage Message}.
+
+(* This relation states that an environment can be split into two environments **)
+Inductive EnvironmentSplit : Env -> Env -> Env -> Prop :=
+  | EnvSplitNil : EnvironmentSplit nil nil nil
+  | EnvSplitNone : forall env1 env2 env,
+      EnvironmentSplit env1 env2 env ->
+      EnvironmentSplit (None :: env1) (None :: env2) (None :: env)
+  | EnvSplitLeft : forall env1 env2 env x,
+      EnvironmentSplit env1 env2 env ->
+      EnvironmentSplit (Some x :: env1) (None :: env2) (Some x :: env)
+  | EnvSplitRight : forall env1 env2 env x,
+      EnvironmentSplit env1 env2 env ->
+      EnvironmentSplit (None :: env1) (Some x :: env2) (Some x :: env).
+
+Lemma EnvironmentSplit_elems : forall env env1 env2,
+  EnvironmentSplit env1 env2 env ->
+  forall x, In (Some x) env <-> (In (Some x) env1) \/ (In (Some x) env2).
+Proof.
+  intros * Split.
+  induction Split; simpl.
+  - intuition.
+  - simpl. intros x.
+    split.
+    + intros [xNone | xIn].
+      * discriminate xNone.
+      * apply IHSplit in xIn.
+        destruct xIn as [In1 | In2].
+        -- left. now right.
+        -- right. now right.
+    + intros [[xNone | xIn] | [xNone | xIn]];
+      try (now left).
+      * assert (In' : In (Some x) env1 \/ In (Some x) env2). now left.
+        rewrite <- IHSplit in In'.
+        now right.
+      * assert (In' : In (Some x) env1 \/ In (Some x) env2). now right.
+        rewrite <- IHSplit in In'.
+        now right.
+  - intros y; split.
+    + intros [ySome | yIn].
+      * left; now left.
+      * rewrite IHSplit in yIn.
+        destruct yIn as [In1 | In2]; intuition.
+    + intros [[ySome | yIn] | [yNone | yIn]].
+      * now left.
+      * assert (In' : In (Some y) env1 \/ In (Some y) env2). now left.
+        rewrite <- IHSplit in In'.
+        intuition.
+      * discriminate yNone.
+      * assert (In' : In (Some y) env1 \/ In (Some y) env2). now right.
+        rewrite <- IHSplit in In'.
+        intuition.
+  - intros y; split.
+    + intros [ySome | yIn].
+      * right; now left.
+      * rewrite IHSplit in yIn.
+        destruct yIn as [In1 | In2]; intuition.
+    + intros [[ySome | yIn] | [yNone | yIn]].
+      * now left.
+      * assert (In' : In (Some y) env1 \/ In (Some y) env2). now left.
+        rewrite <- IHSplit in In'.
+        intuition.
+      * now left.
+      * assert (In' : In (Some y) env1 \/ In (Some y) env2). now right.
+        rewrite <- IHSplit in In'.
+        intuition.
+Qed.
+
+End environment_test.
+
+Notation "Env1 ,, Env2 ~= Env" := (EnvironmentSplit Env1 Env2 Env) (at level 80) : environment_scope.
+
 Section environment_properties.
 
 Context `{M : IMessage Message}.
+
+Lemma EnvironmentSplit_EmptyEnv : forall env, EmptyEnv env -> env,, env ~= env.
+Proof.
+  induction env.
+  - constructor.
+  - intros Empty; inversion Empty; subst; constructor; now apply IHenv.
+Qed.
+
+Lemma EnvironmentSplit_create_EmptyEnv : forall env,
+  env,, create_EmptyEnv env ~= env.
+Proof.
+  induction env.
+  - constructor.
+  - simpl; destruct a.
+    + now apply EnvSplitLeft.
+    + now apply EnvSplitNone.
+Qed.
+
+Lemma EmptyEnv_lookup : forall env, EmptyEnv env -> (forall x, lookup x env = None).
+Proof.
+  induction env; simpl.
+  - intros Empty x; now destruct x.
+  - intros Empty x.
+    inversion Empty; subst.
+    destruct x; simpl.
+    + easy.
+    + now apply IHenv.
+Qed.
+
+Lemma lookup_nil : forall x, lookup x [] = None.
+Proof.
+  now destruct x.
+Qed.
+
+Lemma lookup_False_cons : forall env,
+ (forall x, False <-> is_Some (lookup x (None :: env))) ->
+ (forall x, False <-> is_Some (lookup x env)).
+Proof.
+  intros * Eq x.
+  now generalize (Eq (S x)).
+Qed.
+
+Lemma lookup_False_cons_Some : forall env T,
+  (forall x, 0 = x \/ False <-> is_Some (lookup x (Some T :: env))) ->
+  (forall x, False <-> is_Some (lookup x env)).
+Proof.
+  intros * Eq x.
+  generalize (Eq (S x)).
+  intros EqX.
+  destruct x.
+  - intuition. discriminate H0.
+  - intuition. discriminate H0.
+Qed.
+
+(* TODO: Merge both lemmas into one *)
+Lemma lookup_False_EmptyEnv : forall env, (forall x, False <-> is_Some (lookup x env)) -> EmptyEnv env.
+Proof.
+  induction env; intros Eq.
+  - constructor.
+  - destruct a.
+    + generalize (Eq 0); simpl; intuition.
+    + constructor.
+      reflexivity.
+      apply IHenv. now apply lookup_False_cons.
+Qed.
+
+Lemma lookup_False_EmptyEnv' : forall env, EmptyEnv env -> (forall x, False <-> is_Some (lookup x env)) .
+Proof.
+  induction env; intros Empty.
+  - intros x; now rewrite lookup_nil.
+  - destruct a.
+    + inversion Empty; subst; discriminate.
+    + intros x; inversion Empty; subst.
+      induction x.
+      * easy.
+      * simpl. now apply IHenv.
+Qed.
+
+Lemma lookup_False_SingletonEnv : forall env n,
+  (forall x, n = x \/ False <-> is_Some (lookup x env)) -> SingletonEnv env.
+Proof.
+  induction env; intros * Eq.
+  - induction n.
+    + generalize (Eq 0); rewrite lookup_nil; intuition.
+    + apply IHn.
+      intros x.
+      generalize (Eq (S x)). simpl.
+      intros Eq'.
+      rewrite lookup_nil.
+      assert (H : S n = S x <-> n = x). lia.
+      rewrite H in Eq'.
+      assumption.
+  - induction n.
+    + destruct a.
+      * generalize (lookup_False_cons_Some env t Eq).
+        intros Eq'.
+        simpl.
+        now apply lookup_False_EmptyEnv.
+      * generalize (Eq 0); simpl; intuition.
+    + simpl.
+      destruct a; simpl in *.
+      * apply IHn.
+        generalize (Eq 0).
+        assert (H : S n = 0 <-> False). lia.
+        simpl; rewrite H; intuition.
+      * apply IHenv with (n := n).
+        intros x.
+        generalize (Eq (S x)). simpl.
+        intros Eq'.
+        assert (H : S n = S x <-> n = x). lia.
+        now rewrite <- H.
+Qed.
+
+Lemma lookup_False_n : forall env n,
+  (forall x : nat, n = x \/ False <-> is_Some (lookup x env)) ->
+  exists T, lookup n env = Some T.
+Proof.
+  induction env; intros * Eq.
+  - induction n.
+    + generalize (Eq 0); simpl; intuition.
+    + generalize (Eq (S n)). simpl. intuition.
+  - induction n; simpl in *.
+    + destruct a; simpl in *.
+      * now exists t.
+      * generalize (Eq 0); simpl. intuition.
+    + destruct a; simpl in *.
+      * generalize (Eq 0); simpl.
+        assert (F : S n = 0 <-> False). lia.
+        rewrite F; intuition.
+      * apply IHenv.
+        intros x.
+        generalize (Eq (S x)); simpl; intro Eq'.
+        assert (H : S n = S x <-> n = x). lia.
+        now rewrite <- H.
+Qed.
+
+
+Lemma lookup_cons_None : forall x env T,
+  lookup x (None :: env) = Some T ->
+  lookup (x-1) env = Some T.
+Proof.
+  destruct x; simpl; intros * xLookup.
+  - inversion xLookup.
+  - now rewrite PeanoNat.Nat.sub_0_r.
+Qed.
+
+Lemma lookup_cons_None' : forall x env,
+  x <> 0 ->
+  lookup x (None :: env) = lookup (x-1) env.
+Proof.
+  destruct x; simpl; intros * xLookup.
+  - intuition.
+  - now rewrite PeanoNat.Nat.sub_0_r.
+Qed.
+
+Lemma SingletonEnv_lookup_eq : forall env x y T T',
+  SingletonEnv env ->
+  lookup x env = Some T ->
+  lookup y env = Some T' ->
+  x = y /\ T = T'.
+Proof.
+  intros * Singleton xLookup yLookup.
+  revert x y xLookup yLookup.
+  induction env.
+  - inversion Singleton.
+  - simpl in *.
+    destruct a.
+    + intros * xLookup yLookup.
+      generalize (EmptyEnv_lookup env Singleton).
+      intros nLookup.
+      induction x, y; simpl in *;
+      try (generalize (nLookup x); intros F; now rewrite F in xLookup);
+      try (generalize (nLookup y); intros F; now rewrite F in yLookup);
+      rewrite xLookup in yLookup; now inversion yLookup.
+    + intros * xLookup yLookup.
+      induction x,y; simpl in *;
+      try (discriminate xLookup || discriminate yLookup).
+      simpl in *; generalize (IHenv Singleton x y xLookup yLookup).
+      intros [Eq1 Eq2]; split.
+      * now f_equal.
+      * assumption.
+Qed.
+
+Lemma SingletonEnv_lookup_None : forall env x T,
+  SingletonEnv env ->
+  lookup x env = Some T ->
+  forall y, x <> y -> lookup y env = None.
+Proof.
+  induction env.
+  - intuition; inversion H.
+  - simpl. intros * Single Lookup.
+    destruct a; simpl in *.
+    + assert (H : x = 0).
+      {
+        induction x.
+        - reflexivity.
+        - simpl in *.
+          apply EmptyEnv_lookup with (x := x) in Single.
+          rewrite Single in Lookup.
+          discriminate.
+      }
+      subst; simpl in *.
+      intros ? Neq.
+      destruct y. intuition.
+      simpl.
+      now apply EmptyEnv_lookup.
+    + intros ? Neq.
+      generalize (IHenv (x-1) T Single (lookup_cons_None x env T Lookup)).
+      intros F.
+      destruct y.
+      * reflexivity.
+      * simpl. apply F.
+        intros X.
+        assert (Ge : 0 < x).
+        {
+          induction x.
+          - simpl in Lookup. discriminate.
+          - lia.
+        }
+        lia.
+Qed.
+
+Fixpoint EnvironmentSubtype_diff (env1 env2 : Env) : Env :=
+  match env1, env2 with
+  | nil, nil => nil
+  | None :: env1', None :: env2' => None :: EnvironmentSubtype_diff env1' env2'
+  | Some T :: env1', None :: env2' => Some T :: EnvironmentSubtype_diff env1' env2'
+  | Some T :: env1', Some T' :: env2' => None :: EnvironmentSubtype_diff env1' env2'
+  (* This should never occur when env1 ≤ₑ env2 *)
+  | _, _ => nil
+  end.
+
+Lemma EnvironmentSubtype_diff_CruftEnv : forall env1 env2,
+  env1 ≤ₑ env2 ->
+  CruftEnv (EnvironmentSubtype_diff env1 env2).
+Proof.
+  intros * Sub; induction Sub; simpl; try (now constructor).
+  constructor.
+  now apply Unrestricted_implies_TUCruft.
+  assumption.
+Qed.
+
+Fixpoint EnvironmentSubtype_diff_Sub (env1 env2 : Env) : Env :=
+  match env1, env2 with
+  | nil, nil => nil
+  | None :: env1', None :: env2' => None :: EnvironmentSubtype_diff_Sub env1' env2'
+  | Some T :: env1', None :: env2' => None :: EnvironmentSubtype_diff_Sub env1' env2'
+  | Some T :: env1', Some T' :: env2' => Some T :: EnvironmentSubtype_diff_Sub env1' env2'
+  (* This should never occur when env1 ≤ₑ env2 *)
+  | _, _ => nil
+  end.
+
+Lemma EnvironmentSubtype_diff_Sub_Empty : forall env1 env2,
+  env1 ≤ₑ env2 ->
+  EmptyEnv env2 ->
+  EmptyEnv (EnvironmentSubtype_diff_Sub env1 env2).
+Proof.
+  intros * Sub Empty.
+  induction Sub; simpl in *.
+  - assumption.
+  - inversion Empty; subst.
+    constructor.
+    assumption.
+    now apply IHSub.
+  - inversion Empty; subst.
+    constructor.
+    assumption.
+    now apply IHSub.
+  - inversion Empty; subst; discriminate.
+Qed.
+
+Lemma EnvironmentSubtype_diff_Sub_Singleton : forall env1 env2,
+  env1 ≤ₑ env2 ->
+  SingletonEnv env2 ->
+  SingletonEnv (EnvironmentSubtype_diff_Sub env1 env2).
+Proof.
+  intros * Sub Single.
+  induction Sub; simpl in *.
+  - inversion Single.
+  - now apply IHSub.
+  - now apply IHSub.
+  - now apply EnvironmentSubtype_diff_Sub_Empty.
+Qed.
+
+Lemma EnvironmentSubtype_diff_Sub_lookup : forall env1 env2 v T,
+  env1 ≤ₑ env2 ->
+  lookup v env2 = Some T ->
+  exists T', lookup v (EnvironmentSubtype_diff_Sub env1 env2) = Some T'.
+Proof.
+  intros * Sub.
+  revert v.
+  induction Sub; simpl in *; intros * Lookup.
+  - rewrite lookup_nil in Lookup; discriminate.
+  - destruct v.
+    + simpl in *. discriminate.
+    + apply lookup_cons_None in Lookup.
+      apply IHSub in Lookup.
+      destruct Lookup as [T' Eq].
+      exists T'.
+      rewrite lookup_cons_None'.
+      assumption.
+      lia.
+  - destruct v.
+    + simpl in *. discriminate.
+    + apply lookup_cons_None in Lookup.
+      apply IHSub in Lookup.
+      destruct Lookup as [T' Eq].
+      exists T'.
+      rewrite lookup_cons_None'.
+      assumption.
+      lia.
+  - destruct v.
+    + now exists T1.
+    + simpl in *. now apply IHSub.
+Qed.
+
+(* TODO: Remove this if not needed *)
+
+(*Fixpoint size (env : Env) : nat :=*)
+(*  match env with*)
+(*  | nil => 0*)
+(*  | Some _ :: env' => S (size env')*)
+(*  | None :: env' => size env'*)
+(*  end.*)
+(**)
+(*Definition TTest (x y : option TUsage) :=*)
+(*  match x with*)
+(*  | Some x' => match y with*)
+(*               | Some y' => x' ≤ y'*)
+(*               | None => Unrestricted x'*)
+(*               end*)
+(*  | None => match y with*)
+(*               | Some y' => False*)
+(*               | None => True*)
+(*               end*)
+(*  end.*)
+(**)
+(*Lemma Unrestricted_dec : forall T, {Unrestricted T} + {~ Unrestricted T}.*)
+(*Proof.*)
+(*  intros *.*)
+(*  destruct T.*)
+(*  - left; constructor.*)
+(*  - destruct m; destruct m; destruct u;*)
+(*    try (right; unfold not; intros Un; inversion Un; fail).*)
+(*    left; constructor.*)
+(*Qed.*)
+(**)
+(*Fixpoint get_Unrestricted (env : Env) : Env :=*)
+(*  match env with*)
+(*  | nil => nil*)
+(*  | None :: env' => None :: get_Unrestricted env'*)
+(*  | Some T :: env' => if Unrestricted_dec T*)
+(*                      then Some T :: get_Unrestricted env'*)
+(*                      else None :: get_Unrestricted env'*)
+(*  end.*)
+(**)
+(**)
+(*Lemma EnvironmentSubtype_inv : forall env1 env2,*)
+(*  env1 ≤ₑ env2 ->*)
+(*  env1 = env2 \/ size env1 > size env2 \/ Forall2 TTest env1 env2.*)
+(*Proof.*)
+(*  intros * Sub.*)
+(*  induction Sub.*)
+(*  - now left.*)
+(*  - destruct IHSub as [Eq | [Size | Forall]].*)
+(*    + subst. now left.*)
+(*    + simpl. right. now left.*)
+(*    + now repeat right.*)
+(*  - destruct IHSub as [Eq | [Size | Forall]].*)
+(*    + simpl. subst. right. left. constructor.*)
+(*    + simpl. subst. right. left. lia.*)
+(*    + simpl. now repeat right.*)
+(*  - destruct IHSub as [Eq | [Size | Forall]].*)
+(*    + subst. repeat right.*)
+(*      * easy.*)
+(*      (* TODO: Move to own lemma *)*)
+(*      * induction env2.*)
+(*        -- easy.*)
+(*        -- inversion Sub; subst.*)
+(*           ++ constructor. easy. now apply IHenv2.*)
+(*           ++ constructor. easy. now apply IHenv2.*)
+(*    + right. left. simpl. lia.*)
+(*    + now repeat right.*)
+(*Qed.*)
+
+Lemma create_EmptyEnv_EmptyEnv : forall env, EmptyEnv (create_EmptyEnv env).
+Proof.
+  induction env.
+  - constructor.
+  - now constructor.
+Qed.
+
+Lemma EmptyEnv_SubEnv_EmptyEnv : forall env1 env2, EmptyEnv env1 -> env1 ≤ₑ env2 -> EmptyEnv env2.
+Proof.
+  induction env1; intros * Empty Sub.
+  - inversion Sub; subst; constructor.
+  - inversion Sub; subst.
+    + inversion Empty; subst.
+      constructor.
+      reflexivity.
+      now apply IHenv1.
+    + inversion Empty; subst; discriminate.
+    + inversion Empty; subst; discriminate.
+Qed.
+
+Lemma CruftEnv_EmptyEnv : forall env, EmptyEnv env -> CruftEnv env.
+Proof.
+  induction env.
+  - constructor.
+  - intros Empty.
+    inversion Empty; subst; constructor.
+    + easy.
+    + now apply IHenv.
+Qed.
+
+Lemma SubEnv_EmptyEnv_create_EmptyEnv : forall env,
+  EmptyEnv env ->
+  env ≤ₑ create_EmptyEnv env.
+Proof.
+  intros * Empty; induction env.
+  - constructor.
+  - inversion Empty; subst; constructor; now apply IHenv.
+Qed.
+
+Lemma EnvironmentSubtypeStrict_refl : forall env, env ≼ₑ env.
+Proof.
+  induction env.
+  - constructor.
+  - destruct a; constructor; try (assumption); apply Subtype_refl.
+Qed.
+
+Lemma EnvironmentSubtype_refl : forall env, env ≤ₑ env.
+Proof.
+  induction env.
+  - constructor.
+  - destruct a; constructor; try (apply Subtype_refl || assumption).
+Qed.
 
 End environment_properties.
