theories/TypingRules.v
@@ -6,7 +6,7 @@ From MailboxTypes Require Export Message.
 From MailboxTypes Require Export Syntax.
 From MailboxTypes Require Import Util.
 
-Require Import Lists.List.
+From Stdlib Require Import Lists.List.
 Import ListNotations.
 
 Section typing_rules_def.
@@ -17,7 +17,7 @@ Context `{D : IDefinitionName DefinitionName}.
 
 Inductive WellTypedTerm (prog : Prog) : Env -> Term -> TUsage -> Prop :=
   (* Var *)
-  | VAR   : forall v env T,
+| VAR   : forall v env T,
       SingletonEnv env ->
       lookup v env = Some T ->
       WellTypedTerm prog env (TValue (ValueVar (Var v))) T
@@ -105,13 +105,147 @@ Inductive WellTypedProgram (prog : Prog) : Prop :=
     (forall def, WellTypedDefinition prog (definitions prog def)) ->
     WellTypedTerm prog nil (initialTerm prog) (TUBase BTUnit) -> WellTypedProgram prog.
 
+  Scheme WellTypedTerm_ind_test := Induction for WellTypedTerm Sort Prop.
+  Print WellTypedTerm_ind_test.
+
+  Scheme WellTypedTerm_ind3 := Minimality for WellTypedTerm Sort Prop
+    with WellTypedGuards_ind3 := Minimality for WellTypedGuards Sort Prop
+    with WellTypedGuard_ind3 := Minimality for WellTypedGuard Sort Prop.
+
+  Print WellTypedTerm_ind3.
+
 End typing_rules_def.
+
+Section well_typed_ind'.
+
+  Generalizable All Variables.
+  Context `{M : IMessage Message}.
+  Context `{D : IDefinitionName DefinitionName}.
+
+  Variables (p : Prog).
+  Variable P : Env -> Term -> TUsage -> Prop.
+  Variable PGs : Env -> list Guard -> TUsage -> MPattern -> Prop.
+  Variable PG : Env -> Guard -> TUsage -> MPattern -> Prop.
+
+  Hypothesis VAR_case : forall v env T,
+    SingletonEnv env ->
+    lookup v env = Some T ->
+    P env (TValue (ValueVar (Var v))) T.
+  Hypothesis TRUE_case : forall env,
+    EmptyEnv env -> P env (TValue (ValueBool true)) (TUBase BTBool).
+  Hypothesis FALSE_case : forall env,
+    EmptyEnv env -> P env (TValue (ValueBool false)) (TUBase BTBool).
+  Hypothesis UNIT_case : forall env,
+    EmptyEnv env -> P env (TValue (ValueUnit)) (TUBase BTUnit).
+  Hypothesis APP_case : forall env envList vList definition bodyType argumentTypes term,
+    definitions p definition = FunDef definition argumentTypes bodyType term ->
+    [envList]+ₑ ~= env ->
+    Forall3 P envList (map TValue vList) argumentTypes ->
+    P env (TApp definition vList) bodyType.
+  Hypothesis LET_case : forall (env env1 env2 : Env) (T1 : TType) (T2 : TUsage) (t1 t2 : Term),
+    env1 ▷ₑ env2 ~= env ->
+    P env1 t1 ⌊ T1 ⌋ ->
+    P (Some ⌊ T1 ⌋ :: env2) t2 T2 ->
+    P env (TLet t1 t2) T2.
+  Hypothesis SPAWN_case : forall env t,
+      P env t (TUBase BTUnit) ->
+      P ⌈ env ⌉ₑ (TSpawn t) (TUBase BTUnit).
+  Hypothesis NEW_case : forall env,
+      EmptyEnv env ->
+      P env TNew (? 𝟙 ^^ •).
+  Hypothesis SEND_case : forall env env' envList tList vList m v,
+      P env' (TValue v) (! « m » ^^ ◦) ->
+      signature p m = tList ->
+      [ (env' :: envList) ]+ₑ ~= env ->
+      Forall3 P envList (map TValue vList) (map secondType tList) ->
+      P env (TSend v m vList) (TUBase BTUnit).
+  Hypothesis GUARD_case : forall env env1 env2 guards v T e f,
+      env1 +ₑ env2 ~= env ->
+      P env1 (TValue v) (? f ^^ •) ->
+      PGs env2 guards T f ->
+      e ⊑ f ->
+      f ⊧ f ->
+      P env (TGuard v e guards) T.
+  Hypothesis SUB_case : forall t env1 env2 T1 T2,
+      env1 ≤ₑ env2 ->
+      T1 ≤ T2 ->
+      P env2 t T1 ->
+      P env1 t T2.
+  Hypothesis SINGLE_case : forall T e env g,
+      PG env g T e ->
+      PGs env (g :: nil) T e.
+  Hypothesis SEQ_case : forall T e es env guards g,
+      PG env g T e ->
+      PGs env guards T es ->
+      PGs env (g :: guards) T (e ⊕ es).
+  Hypothesis FAIL_case : forall t env, PG env GFail t 𝟘.
+  Hypothesis FREE_case : forall t env T,
+      P env t T ->
+      PG env (GFree t) T 𝟙.
+  Hypothesis RECEIVE_case : forall t m env T tList e mailbox,
+      signature p m = tList ->
+      BaseTypes tList \/ BaseEnv env ->
+      P ((toEnv (map secondType tList)) ++ [Some (? e ^^ •)] ++ env) t T ->
+      PG env (GReceive m mailbox t) T (« m » ⊙ e).
+
+  Definition WellTypedTerm_ind' : forall {env t T}, WellTypedTerm p env t T -> P env t T.
+  Proof.
+    refine(
+      fix F {env t T} (WT : WellTypedTerm p env t T) : P env t T :=
+        match WT in (WellTypedTerm _ env' t' T') return (P env' t' T') with
+        | VAR _ v env T Single Lookup => VAR_case v env T Single Lookup
+        | TRUE _ env Empty => TRUE_case env Empty
+        | FALSE _ env Empty => FALSE_case env Empty
+        | UNIT _ env Empty => UNIT_case env Empty
+        | APP _ env envList vList def bT aT t L Dis F3 =>
+            APP_case env envList vList def bT aT t L Dis
+              ((fix F3_ind {envList2 vList2 aT2} (F3_WT : Forall3 _ envList2 vList2 aT2) {struct F3_WT} : Forall3 P envList2 vList2 aT2 :=
+                 match F3_WT in (Forall3 _ envList' vList' aT') return (Forall3 P envList' vList' aT') with
+                 | Forall3_nil _ => Forall3_nil _
+                 | Forall3_cons _ t' T' WT' F3' => Forall3_cons _ t' T' (F WT') (F3_ind F3')
+                 end
+              ) envList (map TValue vList) aT F3)
+        | LET _ env env1 env2 T1 T2 t1 t2 Dis WT1 WT2 =>
+            LET_case env env1 env2 T1 T2 t1 t2 Dis (F WT1) (F WT2)
+        | SPAWN _ env t WT => SPAWN_case env t (F WT)
+        | NEW _ env Empty => NEW_case env Empty
+        | SEND _ env env' envList tList vList m v WT s Dis F3 =>
+            SEND_case env env' envList tList vList m v (F WT) s Dis
+              ((fix F3_ind {envList2 vList2 tList2} (F3_WT : Forall3 _ envList2 vList2 tList2) {struct F3_WT} : Forall3 P envList2 vList2 tList2 :=
+                 match F3_WT in (Forall3 _ envList' vList' tList') return (Forall3 P envList' vList' tList') with
+                 | Forall3_nil _ => Forall3_nil _
+                 | Forall3_cons _ t' T' WT' F3' => Forall3_cons _ t' T' (F WT') (F3_ind F3')
+                 end
+              ) envList (map TValue vList) (map secondType tList) F3)
+        | GUARD _ env env1 env2 guards v T e f Dis WT WTGs Inc PNF =>
+            GUARD_case env env1 env2 guards v T e f Dis (F WT) (FGs WTGs) Inc PNF
+        | SUB _ t env1 env2 T1 T2 SubEnv Sub WT' => SUB_case _ _ _ _ _ SubEnv Sub (F WT')
+        end
+      with FGs {env gs T e} (WTGs : WellTypedGuards p env gs T e) : PGs env gs T e :=
+        match WTGs in (WellTypedGuards _ env' gs' T' e') return (PGs env' gs' T' e') with
+        | SINGLE _ _ _ _ _ WTG' => SINGLE_case _ _ _ _ (FG WTG')
+        | SEQ _ _ _ _ _ _ _ WTG' WTGs' => SEQ_case _ _ _ _ _ _ (FG WTG') (FGs WTGs')
+        end
+      with FG {env g T e} (WTG : WellTypedGuard p env g T e) : PG env g T e :=
+        match WTG in (WellTypedGuard _ env' g' T' e') return (PG env' g' T' e') with
+        | FAIL _ env t => FAIL_case env t
+        | FREE _ t env T WT' => FREE_case t env T (F WT')
+        | RECEIVE _ _ _ _ _ _ _ _ s Base WT' => RECEIVE_case _ _ _ _ _ _ _ s Base (F WT')
+        end
+      for F
+    ).
+  Defined.
+
+End well_typed_ind'.
+
 
 Section well_typed_def.
 
 Generalizable All Variables.
 Context `{M : IMessage Message}.
 Context `{D : IDefinitionName DefinitionName}.
+
+(* TODO: Move to environment file *)
 
 (** The domain of an environment is equal to the free variables in a term *)
 Definition EnvEqFV (env : Env) (m : Term) :=
@@ -122,21 +256,348 @@ Definition EnvEqFV (env : Env) (m : Term) :=
    the environment and the domain of the environment is equal to the
    free variables in the term.
 *)
-Definition Cruftless (env : Env) (m : Term) :=
-  forall {T p}, WellTypedTerm p env m T /\ EnvEqFV env m.
+Definition Cruftless {p : Prog} (env : Env) (m : Term) :=
+  exists T, WellTypedTerm p env m T /\ EnvEqFV env m.
+
+Lemma WT_empty_Var : forall p v T, ~ WellTypedTerm p [] (TValue (ValueVar (Var v))) T.
+Proof.
+  intros * WT.
+  remember (TValue (ValueVar (Var v))) as V.
+  remember [] as E.
+  induction WT; try (discriminate HeqV).
+  + subst. inversion H.
+  + subst. inversion H; subst.
+    now apply IHWT.
+Qed.
+
+Lemma not_EmptyEnv_and_SingletonEnv : forall env,
+  ~ (EmptyEnv env /\ SingletonEnv env).
+Proof.
+  induction env.
+  - simpl. intuition.
+  - simpl. destruct a.
+    + intros [Empty1 _]. inversion Empty1; subst. discriminate.
+    + assert (EmptyEnv (None :: env) <-> EmptyEnv env).
+      {
+        split.
+        - intros H; now inversion H.
+        - intros H; now constructor.
+      }
+      now rewrite H.
+Qed.
+
+Lemma WT_EmptyEnv_Var : forall p v T env,
+  EmptyEnv env ->
+  ~ WellTypedTerm p env (TValue (ValueVar (Var v))) T.
+Proof.
+  intros * Empty WT.
+  remember (TValue (ValueVar (Var v))) as V.
+  induction WT; try (discriminate HeqV).
+  + induction env.
+    * inversion H.
+    * destruct a.
+      -- inversion Empty; subst; discriminate.
+      -- now apply not_EmptyEnv_and_SingletonEnv with (env := None :: env).
+  + subst; apply IHWT.
+    * now apply EmptyEnv_SubEnv_EmptyEnv with (env1 := env1).
+    * reflexivity.
+Qed.
+
+Lemma EnvironmentSubtype_diff_Sub_Cruftless_Value : forall p env1 env2 v,
+  env1 ≤ₑ env2 ->
+  @Cruftless p env2 (TValue v) ->
+  @Cruftless p (EnvironmentSubtype_diff_Sub env1 env2) (TValue v).
+Proof.
+  intros * Sub Cruftl.
+  unfold Cruftless in *.
+  destruct Cruftl as [T [WT Eq]].
+  unfold EnvEqFV in *.
+  remember (TValue v) as V.
+  revert env1 Sub.
+  induction WT; intros * Sub; simpl in *; try (discriminate).
+  - destruct v; try discriminate.
+    generalize (EnvironmentSubtype_diff_Sub_lookup env1 env v0 T Sub H0).
+    intros [T' Lookup].
+    exists T'; split.
+    + constructor.
+      now apply EnvironmentSubtype_diff_Sub_Singleton.
+      assumption.
+    + intros x.
+      destruct (PeanoNat.Nat.eq_dec v0 x).
+      * subst; intuition; now rewrite Lookup.
+      * eapply SingletonEnv_lookup_None with (y := x) in Lookup.
+        rewrite Lookup; intuition.
+        now apply EnvironmentSubtype_diff_Sub_Singleton.
+        assumption.
+  - exists (TUBase BTBool); split.
+    + constructor; now apply EnvironmentSubtype_diff_Sub_Empty.
+    + generalize (EnvironmentSubtype_diff_Sub_Empty env1 env Sub H).
+      intros Empty x; apply EmptyEnv_lookup with (x := x) in Empty; now rewrite Empty.
+  - exists (TUBase BTBool); split.
+    + constructor; now apply EnvironmentSubtype_diff_Sub_Empty.
+    + generalize (EnvironmentSubtype_diff_Sub_Empty env1 env Sub H).
+      intros Empty x; apply EmptyEnv_lookup with (x := x) in Empty; now rewrite Empty.
+  - exists (TUBase BTUnit); split.
+    + constructor; now apply EnvironmentSubtype_diff_Sub_Empty.
+    + generalize (EnvironmentSubtype_diff_Sub_Empty env1 env Sub H).
+      intros Empty x; apply EmptyEnv_lookup with (x := x) in Empty; now rewrite Empty.
+  - subst. simpl in *. destruct v; simpl in *.
+    + apply lookup_False_EmptyEnv in Eq; exists (TUBase BTBool); split.
+      * destruct b; constructor; apply EnvironmentSubtype_diff_Sub_Empty; assumption.
+      * apply lookup_False_EmptyEnv'; now apply EnvironmentSubtype_diff_Sub_Empty.
+    + apply lookup_False_EmptyEnv in Eq; exists (TUBase BTUnit); split.
+      * constructor; now apply EnvironmentSubtype_diff_Sub_Empty.
+      * apply lookup_False_EmptyEnv'; now apply EnvironmentSubtype_diff_Sub_Empty.
+    + destruct v. simpl in *.
+      generalize (lookup_False_SingletonEnv env1 n Eq).
+      intros Singleton.
+      generalize (EnvironmentSubtype_diff_Sub_Singleton _ _ Sub Singleton).
+      intros Singleton'.
+      apply lookup_False_n in Eq.
+      destruct Eq as [T Lookup].
+      generalize (EnvironmentSubtype_diff_Sub_lookup _ _ _ _ Sub Lookup).
+      intros [T' Lookup'].
+      exists T'; split.
+      * constructor; assumption.
+      * intros x.
+        destruct (PeanoNat.Nat.eq_dec n x).
+        -- subst; rewrite Lookup'; simpl; intuition.
+        -- generalize (SingletonEnv_lookup_None _ _ _ Singleton' Lookup' _ n0).
+           intros ->; simpl. intuition.
+Qed.
+
+Lemma EnvironmentSubtype_diff_Sub_Cruftless : forall p env1 env2 t,
+  env1 ≤ₑ env2 ->
+  @Cruftless p env2 t ->
+  @Cruftless p (EnvironmentSubtype_diff_Sub env1 env2) t.
+Proof.
+  intros * Sub Cruftl.
+  unfold Cruftless in *.
+  destruct Cruftl as [T [WT Eq]].
+  unfold EnvEqFV in *.
+  induction WT; simpl in *.
+  - generalize (EnvironmentSubtype_diff_Sub_lookup env1 env v T Sub H0).
+    intros [T' Lookup].
+    exists T'; split.
+    + constructor.
+      now apply EnvironmentSubtype_diff_Sub_Singleton.
+      assumption.
+    + intros x.
+      destruct (PeanoNat.Nat.eq_dec v x).
+      * subst; intuition; now rewrite Lookup.
+      * eapply SingletonEnv_lookup_None with (y := x) in Lookup.
+        rewrite Lookup; intuition.
+        now apply EnvironmentSubtype_diff_Sub_Singleton.
+        assumption.
+  - exists (TUBase BTBool); split.
+    + constructor; now apply EnvironmentSubtype_diff_Sub_Empty.
+    + generalize (EnvironmentSubtype_diff_Sub_Empty env1 env Sub H).
+      intros Empty x; apply EmptyEnv_lookup with (x := x) in Empty; now rewrite Empty.
+  - exists (TUBase BTBool); split.
+    + constructor; now apply EnvironmentSubtype_diff_Sub_Empty.
+    + generalize (EnvironmentSubtype_diff_Sub_Empty env1 env Sub H).
+      intros Empty x; apply EmptyEnv_lookup with (x := x) in Empty; now rewrite Empty.
+  - exists (TUBase BTUnit); split.
+    + constructor; now apply EnvironmentSubtype_diff_Sub_Empty.
+    + generalize (EnvironmentSubtype_diff_Sub_Empty env1 env Sub H).
+      intros Empty x; apply EmptyEnv_lookup with (x := x) in Empty; now rewrite Empty.
+  - admit.
+  - admit.
+  - admit.
+  - admit.
+  - admit.
+  - admit.
+  - exists T2; split.
+    + eapply SUB.
+      * admit.
+      * exact H0.
+      * exact WT.
+    + fold (EnvEqFV env0 t) in Eq.
+Admitted.
+
+Lemma ValueVar_Cruftless : forall {p} env v T,
+  SingletonEnv env ->
+  lookup v env = Some T ->
+  @Cruftless p env (TValue (ValueVar (Var v))).
+Proof.
+  intros * Singleton Lookup.
+  unfold Cruftless.
+  exists T.
+  split.
+  - now constructor.
+  - intros x.
+    simpl.
+    intuition.
+    + unfold is_Some. subst. now rewrite Lookup.
+    + destruct (lookup x env) eqn:xLookup.
+      * generalize (SingletonEnv_lookup_eq env v x T t Singleton Lookup xLookup).
+        intuition.
+      * intuition.
+Qed.
+
+Lemma stes : forall env T,
+  (forall x, 0 = x \/ False <-> is_Some (lookup x (Some T :: env))) ->
+  (forall x, False <-> is_Some (lookup x env)).
+Proof.
+  intros * Eq x.
+  generalize (Eq (S x)).
+  intros EqX.
+  destruct x.
+  - intuition. discriminate H0.
+  - intuition. discriminate H0.
+Qed.
+
+Lemma stes' : forall env n T,
+  (forall x, n = x \/ False <-> is_Some (lookup x (Some T :: env))) ->
+  n = 0.
+Proof.
+  induction n; intros * Eq.
+  - reflexivity.
+  - generalize (Eq 0); simpl; intuition.
+Qed.
+
+Lemma canonical_form_BTBool : forall {p} env v,
+  WellTypedTerm p env (TValue v) (TUBase BTBool) ->
+  v = ValueBool false \/ v = ValueBool true \/ exists n, v = ValueVar (Var n).
+Proof.
+  intros * WT.
+  remember (TUBase BTBool) as T.
+  destruct v.
+  - destruct b; intuition.
+  - remember (TValue ValueUnit) as V.
+    induction WT; try (discriminate HeqV); try (discriminate HeqT).
+    subst.
+    apply Subtype_inversion_TUBase_right in H0.
+    now apply IHWT.
+  - remember (TValue (ValueVar v)) as V.
+    induction WT; try (discriminate HeqT); try (discriminate HeqV).
+    + repeat right. exists v0. now inversion HeqV.
+    + subst.
+      apply Subtype_inversion_TUBase_right in H0.
+      now apply IHWT.
+Qed.
+
+Lemma canonical_form_BTUnit : forall {p} env v,
+  WellTypedTerm p env (TValue v) (TUBase BTUnit) ->
+  v = ValueUnit \/ exists n, v = ValueVar (Var n).
+Proof.
+  intros * WT.
+  remember (TUBase BTUnit) as T.
+  remember (TValue v) as V.
+  induction WT; try (discriminate HeqT); try (discriminate HeqV).
+  + right; exists v0; now inversion HeqV.
+  + left; now inversion HeqV.
+  + subst; apply Subtype_inversion_TUBase_right in H0; now apply IHWT.
+Qed.
+
+Lemma test' : forall vList tList t,
+  t :: tList = map TValue vList ->
+  exists v vList', t = TValue v /\ tList = map TValue vList'.
+Proof.
+  induction vList; simpl; intros * Eq.
+  - discriminate Eq.
+  - inversion Eq.
+    now exists a, vList.
+Qed.
+
+Lemma lookup_None : forall n env T,
+  lookup n (None :: env) = Some T -> lookup (n-1) env = Some T.
+Proof.
+  intros n.
+  induction env; simpl; intros * Eq.
+  - induction n; simpl in *.
+    + discriminate.
+    + rewrite lookup_nil in Eq; discriminate.
+  - induction n; simpl in *.
+    + discriminate.
+    + replace (n-0) with n. assumption.
+      now destruct n.
+Qed.
+
+Lemma WellTypedEnvSub_TValueVar :
+  forall {T p} env v,
+  WellTypedTerm p env (TValue (ValueVar (Var v))) T ->
+  exists env1 env2 env3 T',
+    env1,, env2 ~= env /\
+    T' ≤ T /\
+    WellTypedTerm p env3 (TValue (ValueVar (Var v))) T' /\
+    @Cruftless p env1 (TValue (ValueVar (Var v))) /\
+    env1 ≼ₑ env3 /\
+    CruftEnv env2.
+Proof.
+  intros * WT.
+  remember (TValue (ValueVar (Var v))) as V.
+  induction WT; try (subst; discriminate).
+  - inversion HeqV. subst.
+    exists env, (create_EmptyEnv env), env, T.
+    repeat split.
+    + apply EnvironmentSplit_create_EmptyEnv.
+    + apply Subtype_refl.
+    + now constructor.
+    + now apply ValueVar_Cruftless with (T := T).
+    + apply EnvironmentSubtypeStrict_refl.
+    + apply CruftEnv_EmptyEnv; apply create_EmptyEnv_EmptyEnv.
+  - subst.
+    generalize (IHWT eq_refl).
+    intros [env1' [env2' [env3' [T' [Split [Sub [WT' [Cruftless' [SubStrict Cruft']]]]]]]]].
+    clear IHWT.
+    generalize (EnvironmentSubtype_diff_CruftEnv env1 env2 H). intros.
+    exists env1', env2', env3', T'.
+    repeat split.
+    + admit.
+    + eapply Subtype_trans. apply Sub. assumption.
+    + assumption.
+    + assumption.
+    + assumption.
+    + assumption.
+Admitted.
+
+Lemma xfy : forall p env b T, WellTypedTerm p env (TValue (ValueBool b)) T -> T = TUBase BTBool.
+Proof.
+  intros * WT.
+  remember (TValue (ValueBool b)) as V.
+  induction WT; try (discriminate HeqV).
+  - reflexivity.
+  - reflexivity.
+  - generalize (IHWT HeqV).
+    intros ->.
+    now apply Subtype_inversion_TUBase_left in H0.
+Qed.
+
+Lemma WellTypedEnvSub_TValue :
+  forall {T p} env v,
+  WellTypedTerm p env (TValue v) T ->
+  exists env1 env2 env3 T',
+    env1,, env2 ~= env /\
+    T' ≤ T /\
+    WellTypedTerm p env3 (TValue v) T' /\
+    @Cruftless p env1 (TValue v) /\
+    env1 ≼ₑ env3 /\
+    CruftEnv env2.
+Proof.
+Admitted.
+
 
 (** Lemma D.4 *)
 Lemma WellTypedEnvSub :
   forall {T p} env m,
   WellTypedTerm p env m T ->
   exists env1 env2 env3 T',
-    env = env1 ++ env2 /\
+    env1,, env2 ~= env /\
     T' ≤ T /\
     WellTypedTerm p env3 m T' /\
-    @Cruftless env1 m /\
+    @Cruftless p env1 m /\
     env1 ≼ₑ env3 /\
     CruftEnv env2.
 Proof.
+  intros * WT.
+  remember env as E.
+  induction WT.
+  - apply WellTypedEnvSub_TValue; now constructor.
+  - apply WellTypedEnvSub_TValue; now constructor.
+  - apply WellTypedEnvSub_TValue; now constructor.
+  - apply WellTypedEnvSub_TValue; now constructor.
+  -
 Admitted.
 
 End well_typed_def.
